deps/poulet4/lib/P4automata/PreBisimulationSyntax.v
@@ -13,6 +13,28 @@ Module P4A := Poulet4.P4automata.Syntax.
 
 Open Scope list_scope.
 
+Fixpoint n_tuple A (n: nat): Type :=
+  match n with
+  | 0 => unit
+  | S n => n_tuple A n * A
+  end.
+
+Fixpoint t2l A (n: nat) (x: n_tuple A n) : list A :=
+  match n as n' return n_tuple A n' -> list A with
+  | 0 => fun _ => []
+  | S n => fun p => t2l A n (fst p) ++ [snd p]
+  end x.
+
+Lemma split_ex:
+  forall A B (P: A * B -> Prop),
+    (exists x: A, exists y: B, P (x, y)) <->
+    exists x: A * B, P x.
+Proof.
+  firstorder.
+  destruct x.
+  firstorder.
+Qed.
+
 (* Bitstring variable context. *)
 Inductive bctx :=
 | BCEmp: bctx
@@ -25,7 +47,7 @@ Global Instance bctx_eq_dec : EquivDec.EqDec bctx eq := bctx_eqdec.
 Fixpoint bval (c: bctx) : Type :=
   match c with
   | BCEmp => unit
-  | BCSnoc c' size => bval c' * {b: list bool | List.length b = size}
+  | BCSnoc c' size => bval c' * n_tuple bool size
   end.
 
 Inductive bvar : bctx -> Type :=
@@ -62,30 +84,8 @@ Fixpoint check_bvar {c} (x: bvar c) : nat :=
   | BVarRest x' => check_bvar x'
   end.
 
-Fixpoint n_tuple A (n: nat): Type :=
-  match n with
-  | 0 => unit
-  | S n => n_tuple A n * A
-  end.
-
-Fixpoint t2l A (n: nat) (x: n_tuple A n) : list A :=
-  match n as n' return n_tuple A n' -> list A with
-  | 0 => fun _ => []
-  | S n => fun p => t2l A n (fst p) ++ [snd p]
-  end x.
-
-Lemma split_ex:
-  forall A B (P: A * B -> Prop),
-    (exists x: A, exists y: B, P (x, y)) <->
-    exists x: A * B, P x.
-Proof.
-  firstorder.
-  destruct x.
-  firstorder.
-Qed.
-
 Equations interp_bvar {c} (valu: bval c) (x: bvar c) : list bool :=
-  { interp_bvar (_, bs)    (BVarTop _ _)  := proj1_sig bs;
+  { interp_bvar (_, bs)    (BVarTop _ _)  := t2l _ _ bs;
     interp_bvar (valu', bs) (BVarRest x')  := interp_bvar valu' x' }.
 
 Section ConfRel.
@@ -401,7 +401,7 @@ Section ConfRel.
   Definition interp_conf_rel (phi: conf_rel) : relation conf :=
     fun x y => 
       (exists (t1: n_tuple _ phi.(cr_st).(cs_st1).(st_buf_len)) 
-             (t2: n_tuple _ phi.(cr_st).(cs_st1).(st_buf_len)),
+         (t2: n_tuple _ phi.(cr_st).(cs_st2).(st_buf_len)),
              t2l _ _ t1 = snd x /\
              t2l _ _ t2 = snd y /\
              interp_conf_state phi.(cr_st) x y) ->
